{
 "cells": [
  {
   "cell_type": "markdown",
   "metadata": {},
   "source": [
    "# AM 205 - Midterm\n",
    "\n",
    "## By Jonathan Guillotte-Blouin"
   ]
  },
  {
   "cell_type": "markdown",
   "metadata": {},
   "source": [
    "### Question 1: A stencil based on least squares\n",
    "\n",
    "#### a) Calculate the coefficients $a_{-1}$, $a_0$, $a_1$, $a_2$, and $a_3$ to make a fourth-order accurate finite-difference formula."
   ]
  },
  {
   "cell_type": "markdown",
   "metadata": {},
   "source": [
    "To do this, we will use the Lagrange interpolant approach.\n",
    "\n",
    "$$ \\mathcal{L_{-1}}(z) = \\frac{(z-kh)(z-kh-h)(z-kh-2h)(z-kh-3h)}{(-h)(-2h)(-3h)(-4h)} = \\frac{(z-kh)(z-kh-h)(z-kh-2h)(z-kh-3h)}{24h^4}$$\n",
    "\n",
    "Assume $\\mathcal{L'_x(z)} = \\frac{\\partial L_x(z)}{\\partial z}$.\n",
    "\n",
    "$$ \\mathcal{L'_{-1}}(0) = -\\frac{2h^3(2k^3 +9k^2+11k+3)}{24h^4} = -\\frac{2k^3 +9k^2+11k+3}{12h}$$\n",
    "\n",
    "$$ \\mathcal{L_{0}}(z) = \\frac{(z-kh+h)(z-kh-h)(z-kh-2h)(z-kh-3h)}{h(-h)(-2h)(-3h)} = \\frac{(z-kh+h)(z-kh-h)(z-kh-2h)(z-kh-3h)}{-6h^4}$$\n",
    "\n",
    "$$ \\mathcal{L'_{0}}(0) = -\\frac{h^3(4k^3 +15k^2+10k-5)}{-6h^4} = \\frac{4k^3 +15k^2+10k-5}{6h}$$\n",
    "\n",
    "\n",
    "$$ \\mathcal{L_{1}}(z) = \\frac{(z-kh+h)(z-kh)(z-kh-2h)(z-kh-3h)}{(2h)h(-h)(-2h)} = \\frac{(z-kh+h)(z-kh)(z-kh-2h)(z-kh-3h)}{4h^4}$$\n",
    "\n",
    "$$ \\mathcal{L'_{1}}(0) = -\\frac{2h^3(2k^3 +6k^2+k-3)}{4h^4} = -\\frac{2k^3 +6k^2+k-3}{2h}$$\n",
    "\n",
    "\n",
    "\n",
    "$$ \\mathcal{L_{2}}(z) = \\frac{(z-kh+h)(z-kh)(z-kh-h)(z-kh-3h)}{(3h)(2h)h(-h)} = \\frac{(z-kh+h)(z-kh)(z-kh-2h)(z-kh-3h)}{-6h^4}$$\n",
    "\n",
    "$$ \\mathcal{L'_{2}}(0) = \\frac{h^3(-4k^3 -9k^2+2k+3)}{-6h^4} = -\\frac{-4k^3 -9k^2+2k+3}{6h}$$\n",
    "\n",
    "\n",
    "$$ \\mathcal{L_{3}}(z) = \\frac{(z-kh+h)(z-kh)(z-kh-h)(z-kh-2h)}{(4h)(3h)(2h)h} = \\frac{(z-kh+h)(z-kh)(z-kh-h)(z-kh-2h)}{24h^4}$$\n",
    "\n",
    "$$ \\mathcal{L'_{3}}(0) = \\frac{-2h^3(2k^3 +3k^2-k-1)}{24h^4} = -\\frac{2k^3 +3k^2-k-1}{12h}$$"
   ]
  },
  {
   "cell_type": "markdown",
   "metadata": {},
   "source": [
    "$$ l'(z) = \\mathcal{L'_{-1}}(z) \\, f_{k-1} + \\mathcal{L'_{0}}(z) \\, f_k + \\mathcal{L'_{1}}(z) \\, f_{k+1} + \\mathcal{L'_{2}}(z) \\, f_{k+2} + \\mathcal{L'_{3}}(z) \\, f_{k+3} $$\n",
    "\n",
    "$$ f'_{diff1}(x_k) = l'(0) = \\frac{-\\frac{2k^3 +9k^2+11k+3}{12} \\, f_{k-1} + \\frac{4k^3 +15k^2+10k-5}{6} \\, f_k -\\frac{2k^3 +6k^2+k-3}{2} \\, f_{k+1} - \\frac{-4k^3 -9k^2+2k+3}{6} \\, f_{k+2} - \\frac{2k^3 +3k^2-k-1}{12} \\, f_{k+3}}{h} $$"
   ]
  },
  {
   "cell_type": "code",
   "execution_count": null,
   "metadata": {},
   "outputs": [],
   "source": []
  }
 ],
 "metadata": {
  "kernelspec": {
   "display_name": "Python 3",
   "language": "python",
   "name": "python3"
  },
  "language_info": {
   "codemirror_mode": {
    "name": "ipython",
    "version": 3
   },
   "file_extension": ".py",
   "mimetype": "text/x-python",
   "name": "python",
   "nbconvert_exporter": "python",
   "pygments_lexer": "ipython3",
   "version": "3.6.5"
  }
 },
 "nbformat": 4,
 "nbformat_minor": 2
}
